\begin{eqntable}{$q$-th projection of $\mathsf{restr}$, or faces\label{tab:faces}}
  \eqnline{\restrf[m][\epsilon][q][n][p][p \leq q \leq n - 1]}{\makecell{(D:\Xto{m}{n}) \\ (d:\framep[m][n][p][][D=\D])}}{:}{\framep[m][n-1][p][][D=\hdD]}

  \eqnline{\restrf[m][\epsilon][q][n][p'+1]}{D~(\pair{d}{l})}{\defeq}{(\restrf[m][\epsilon][q][n][p'][][D=\D, d=\d],\restrl[m][\epsilon][q-1][n][p'][][D=\D, d=\d, l=\l])}

  \\

  \eqnline{\restrl[m][\epsilon][q][n][p][p \leq q \leq n - 2]}{\makecell{(D:\Xto{m}{n}) \\ (d:\framep[m][n][p][][D=\D]) \\ (l:\layer[m][n][p][][D=\D, d=\d])}}{:}{\layer[m][n-1][p][][D=\hdD](\restrf[m][\epsilon][q+1][n][p][][D=\D, d=\d])}

  \eqnline{\restrl[m][\epsilon][q][n,p]}{\D~\d~\l}{\defeq}{\lambda \omega.(\cohf[m][\epsilon][\omega][q][p][n][p][][D=\D, d=\d](\restrc[m][\epsilon][q][n-1][p][][D=\hdD, d=\tlD](\restrf[m][\omega][p][n][p][][D=\D, d=\d])(l_\omega)))}

  \\

  \eqnline{\restrc[m][\epsilon][q][n][p][p \leq q \leq n - 1]}{\makecell{(D:\Xto{m}{n}) \\ (E:\Xcomp{m}{n}[D=\D]) \\(d:\framep[m][n][p][][D=\D]) \\ (c:\filler[m][n][p][][D=\D, E=\E, d=\d])}}{:}{\filler[m][n-1][p][][D=\hdD, d=\tlD](\restrf[m][\epsilon][q+1][n][p][][D=\D, d=\d])}

  \eqnline{\restrc[m][\epsilon][q][n][p][p=q]}{\D~\E~\d~(\pair{l}{\_})}{\defeq}{\l_\epsilon}

  \eqnline{\restrc[m][\epsilon][q][n][p][p<q]}{\D~\E~\d~(\pair{l}{c})}{\defeq}{(\restrl[m][\epsilon][q][n][p][][D=\D, d=\d, l=\l],\restrc[m][\epsilon][q][n][p+1][][D=\D, E=\E, d=\pair{d}{l}, c=\c])}
\end{eqntable}
